cal/example/BQProof.v
@@ -1,9 +1,10 @@
 From Coq Require Import Lia.
 From models Require Import
      IntSpec.
-From examples Require Import
-     CAL CompCertIntSpec RefConv
-     CompCertCAL BoundedQueueCode.
+From cal Require Import
+     CompCertIntSpec RefConv
+     IntSpecCAL CompCertCAL
+     BQ BQCode.
 From lattices Require Import
      Upset Downset FCD.
 From structures Require Import Lattice. (* subrel *)
@@ -19,7 +20,7 @@ Import ListNotations ISpec.
 
 (** * Example: ring buffer and bounded queue *)
 
-Parameter val_rel: CAL.val -> val -> Prop.
+Parameter val_rel: BQ.val -> val -> Prop.
 Hypothesis val_is_int:
   forall c v, val_rel c v -> Cop.val_casted v tint.
 Hint Resolve val_is_int.
@@ -51,7 +52,7 @@ Section MARSHALL.
     Genv.find_symbol se get_id = Some b ->
     c_i = Vint (Integers.Int.repr (Z.of_nat i)) ->
     Ple (Genv.genv_next se) (Mem.nextblock m) ->
-    rb_rc_rel _ (CAL.get i) _ (c_event vf get_sg [ c_i ] se # m) (rel_with_mem val_rel m)
+    rb_rc_rel _ (BQ.get i) _ (c_event vf get_sg [ c_i ] se # m) (rel_with_mem val_rel m)
   | rb_inc1_rel vf b m se:
     vf = Vptr b Integers.Ptrofs.zero ->
     Genv.find_symbol se inc1_id = Some b ->
@@ -77,67 +78,20 @@ Section MARSHALL.
     bq_rc_rel _ deq _ (c_event vf deq_sg [ ] se # m) (rel_with_mem val_rel m).
 
   Local Obligation Tactic := idtac.
-  Program Definition rb_rc : esig_rc rb_sig :=
-    {|
-      esig_refconv := rb_rc_rel;
-    |}.
-  Next Obligation.
-    intros * Hrel Hvf Hvargs.
-    rc_elim (inv) Hrel; unfold mem in *; depsubst; clear_hyp.
-    - apply val_inject_id in Hvf. inv Hvf.
-      inv Hvargs. apply val_inject_id in H1. inv H1.
-      inv H3. apply val_inject_id in H1. inv H1.
-      2: { apply val_is_int in H12. inv H12. }
-      inv H4.
-      eapply refconv_clo. eauto.
-      rc_eapply rb_set_rel; eauto.
-    - apply val_inject_id in Hvf. inv Hvf.
-      inv Hvargs. apply val_inject_id in H1. inv H1.
-      inv H3.
-      eapply refconv_clo. eauto.
-      rc_eapply rb_get_rel; eauto.
-    - apply val_inject_id in Hvf. inv Hvf.
-      inv Hvargs.
-      eapply refconv_clo. eauto.
-      rc_eapply rb_inc1_rel; eauto.
-    - apply val_inject_id in Hvf. inv Hvf.
-      inv Hvargs.
-      eapply refconv_clo. eauto.
-      rc_eapply rb_inc2_rel; eauto.
-  Qed.
+  Definition rb_rc : esig_rc rb_sig :=
+    {| esig_refconv := rb_rc_rel; |}.
 
-  Program Definition bq_rc : esig_rc bq_sig :=
-    {|
-      esig_refconv := bq_rc_rel;
-    |}.
-  Next Obligation.
-    intros * Hrel Hvf Hvargs.
-    rc_elim (inv) Hrel; unfold mem in *; depsubst; clear_hyp.
-    - apply val_inject_id in Hvf. inv Hvf.
-      inv Hvargs. apply val_inject_id in H1. inv H1.
-      2: { apply val_is_int in H11. inv H11. }
-      inv H3.
-      eapply refconv_clo. eauto.
-      rc_eapply bq_enq_rel; eauto.
-    - apply val_inject_id in Hvf. inv Hvf.
-      inv Hvargs.
-      eapply refconv_clo. eauto.
-      rc_eapply bq_deq_rel; eauto.
-  Qed.
+  Definition bq_rc : esig_rc bq_sig :=
+    {| esig_refconv := bq_rc_rel; |}.
 
 End MARSHALL.
 
 Hint Constructors nat_rel void_rel.
 
 Local Opaque fsup finf.
-Local Opaque semantics2 normalize_rc.
+Local Opaque semantics2.
 
 (* Import Ptrofs. *)
-
-Ltac clear_hyp :=
-  repeat match goal with
-         | [ H : (?t = ?t)%type |- _ ] => clear H
-         end.
 
 Section RHO.
 
@@ -147,16 +101,17 @@ Section RHO.
   | R_cnt_intro b v n m:
     Genv.find_symbol se id = Some b ->
     Mem.load Mint32 m b 0 = Some v ->
-    nat_rel n v -> (n < CAL.N)%nat ->
+    nat_rel n v -> (n < BQ.N)%nat ->
     Mem.range_perm m b 0 4 Cur Writable ->
     R_cnt id n m.
 
-  Inductive R_arr : (nat -> CAL.val) -> mem -> Prop :=
+  Inductive R_arr : (nat -> BQ.val) -> mem -> Prop :=
   | R_arr_intro f b m:
     Genv.find_symbol se arr_id = Some b ->
-    (forall i, exists v, Mem.load Mint32 m b (4 * Z.of_nat i) = Some v /\
+    (forall i, (i < BQ.N)%nat ->
+      exists v, Mem.load Mint32 m b (4 * Z.of_nat i) = Some v /\
                  val_rel (f i) v) ->
-    (forall ofs, 0 <= ofs < 4 * Nz + 4 ->
+    (forall ofs, 0 <= ofs < 4 * Nz ->
             Mem.perm m b ofs Cur Writable) ->
     R_arr f m.
 
@@ -170,45 +125,56 @@ End RHO.
 Program Definition rho_rb : rho_rel rb_state :=
   {|
     rho_pred := R_rb;
-    rho_footprint i := i = cnt1_id \/ i = cnt2_id \/ i = arr_id;
+    rho_footprint := (cnt1_id, 4) :: (cnt2_id, 4)
+                       :: (arr_id, Nz * 4) :: nil;
   |}.
 Next Obligation.
   destruct H. constructor.
   - inv H. econstructor; eauto.
     + eapply Mem.load_unchanged_on; eauto.
-      cbn. unfold KRel.blocks. intros.
-      eexists; split; [|eauto]. left. reflexivity.
+      cbn. intros.
+      apply Exists_cons_hd. split; eauto.
     + unfold Mem.range_perm in *. intros ofs Hofs.
       eapply Mem.perm_unchanged_on; eauto.
-      cbn. unfold KRel.blocks. intros.
-      eexists; split; [|eauto]. left. reflexivity.
+      apply Exists_cons_hd. split; eauto.
   - inv H1. econstructor; eauto.
     + eapply Mem.load_unchanged_on; eauto.
-      cbn. unfold KRel.blocks. intros.
-      eexists; split; [|eauto]. right. left. reflexivity.
+      cbn. intros.
+      apply Exists_cons_tl. apply Exists_cons_hd. split; eauto.
     + unfold Mem.range_perm in *. intros ofs Hofs.
       eapply Mem.perm_unchanged_on; eauto.
-      cbn. unfold KRel.blocks. intros.
-      eexists; split; [|eauto]. right. left. reflexivity.
+      apply Exists_cons_tl. apply Exists_cons_hd. split; eauto.
   - inv H2. econstructor; eauto.
-    + intros i. specialize (H4 i) as (v & Hv1 & Hv2).
-      exists v; split; eauto.
+    + intros i Hi. specialize (H4 i) as (v & Hv1 & Hv2).
+      apply Hi. exists v; split; eauto.
       eapply Mem.load_unchanged_on; eauto.
-      unfold KRel.blocks. intros.
-      eexists; split; [|eauto]. right. right. reflexivity.
+      intros.
+      apply Exists_cons_tl. apply Exists_cons_tl.
+      apply Exists_cons_hd. split; eauto.
+      replace (size_chunk Mint32) with 4 in H2 by reflexivity.
+      unfold Nz. lia.
     + unfold Mem.range_perm in *. intros ofs Hofs.
       eapply Mem.perm_unchanged_on; eauto.
-      cbn. unfold KRel.blocks. intros.
-      eexists; split; [|eauto]. right. right. reflexivity.
+      apply Exists_cons_tl. apply Exists_cons_tl.
+      apply Exists_cons_hd. split; eauto. lia.
 Qed.
 Next Obligation.
-  inv H. unfold KRel.blocks in H0.
-  eapply Mem.perm_valid_block with (ofs := 0).
-  destruct H0 as (v & [|[|]] & Hv2).
-  - inv H1. replace b with b0 by congruence. apply H6. lia.
-  - inv H2. replace b with b0 by congruence. apply H6. lia.
-  - inv H3. replace b with b0 by congruence. apply H4.
-    unfold Nz. lia.
+  inv H. eapply Mem.perm_valid_block with (ofs := 0).
+  inv H0. 2: inv H4.
+  - inv H1. destruct H4. replace b with b0 by congruence. apply H7. lia.
+  - inv H2. destruct H0. replace b with b0 by congruence. apply H7. lia.
+  - inv H3. inv H0. destruct H6.
+    replace b with b0 by congruence.
+    apply H5. lia. inv H6.
+Qed.
+Next Obligation.
+  inv H. inv H0. 2: inv H4.
+  - inv H1. destruct H4. replace b with b0 by congruence. eauto with mem.
+  - inv H2. destruct H0. replace b with b0 by congruence. eauto with mem.
+  - inv H3. inv H0. destruct H6.
+    replace b with b0 by congruence.
+    assert (Mem.perm m b0 ofs Cur Writable). apply H5. lia.
+    eauto with mem. inv H6.
 Qed.
 
 (*
@@ -243,8 +209,8 @@ Section RB.
   Hypothesis N_neq_0: Nz <> 0.
 
   Lemma cnt_inc_simp c i:
-    Z.of_nat c = Int.intval i -> (c < CAL.N)%nat ->
-    Z.of_nat (S c mod CAL.N) = Int.intval (Int.modu (Int.add i (Int.repr 1)) (Int.repr Nz)).
+    Z.of_nat c = Int.intval i -> (c < BQ.N)%nat ->
+    Z.of_nat (S c mod BQ.N) = Int.intval (Int.modu (Int.add i (Int.repr 1)) (Int.repr Nz)).
   Proof.
     intros H1 H2. unfold Int.add, Int.modu.
     apply inj_le in H2. rewrite Nat2Z.inj_succ in H2.
@@ -256,7 +222,7 @@ Section RB.
       + f_equal. rewrite Nat2Z.inj_succ. reflexivity.
       + lia.
     - unfold Int.unsigned. rewrite <- H1.
-      exploit (Z.mod_pos_bound (Z.of_nat c + 1) (Z.of_nat CAL.N)); lia.
+      exploit (Z.mod_pos_bound (Z.of_nat c + 1) (Z.of_nat BQ.N)); lia.
   Qed.
 
   Lemma cop_sem_mod m i j:
@@ -272,7 +238,7 @@ Section RB.
 
   Lemma rb_code_correct:
     L_rb [= slift (right_arrow rb_rc)
-         @@ right_arrow (rho_with_se rho_rb)
+         @@ right_arrow (rho_rc rho_rb)
          @ right_arrow c_rc
          @ ang_lts_spec (semantics2 rb_program) @ bot.
   Proof.
@@ -304,14 +270,22 @@ Section RB.
     inf_intro [ Rc Hc ]. intm.
     rc_inversion Hc. depsubst. inv H. inv H0. clear Hrel. rename Hsub into HRc.
     rc_inversion Hrho. unfold rb_state in *. depsubst. clear Hrel. rename Hsub into Hrho.
-    inv H1. rename H into Hm. destruct H0 as [HRst Hperm]. cbn in Hperm.
-    (* rc_elim (inv) H2. depsubst. inv H1. *)
-    (* rc_elim (inv) H13. unfold rb_state in H1. depsubst. inv H2. destruct H0. *)
-    (* rename H into Hm. rename H0 into HRst. rename H1 into Hperm. *)
-    (* rename Hsub into HR1. rename Hsub0 into HR2. *)
+    inv H6. rename H into Hm. rename H12 into Hvdef.
+    rename H13 into Hvinj. rename H14 into Hargs.
+    destruct H0 as [Hperm [Hdef HRst]].
     unfold assume. inf_intro Hse. intm.
     rc_elim (inv) Hr; unfold mem in *; depsubst; clear_hyp.
     - rename H10 into Hb. rename H12 into Hv. rename H13 into Hnb.
+      replace vf' with (Vptr b zero).
+      2: inv Hvinj; inv H1; reflexivity.
+      replace args' with ([Vint (Int.repr (Z.of_nat i2)); c_v]).
+      2: {
+        inv Hargs. f_equal. inv H1. reflexivity.
+        inv H3. f_equal. apply val_is_int in Hv.
+        inv Hv. inv H2. reflexivity. inv H2. inv H4. f_equal.
+        rewrite add_zero. reflexivity.
+        inv H5. reflexivity.
+      }
       apply assert_l. intros Hi. apply inj_lt in Hi.
       setoid_rewrite sup_fsup. sup_mor. eapply fsup_at.
       (* initial state *)
@@ -353,40 +327,61 @@ Section RB.
       { cbn. apply HRc. reflexivity. }
       fcd_simpl. sup_mor. cbn. eapply (fsup_at (Vundef, (mm, (update f i2 v, c1, c2)))).
       {
-        apply Hrho. subst R1. cbn. repeat apply conj; eauto. 2: constructor.
-        + eapply Mem.store_outside_extends; eauto.
-          intros. unfold AbstractStateRel.no_perm_on in Hperm.
-          apply (Hperm b0 ofs'). cbn.
-          unfold KRel.blocks. exists arr_id. split; auto.
-          apply Mem.perm_cur_max.
-          eapply Mem.perm_implies; eauto. apply perm_any_N.
-        + destruct H2. econstructor; eauto.
-          erewrite Mem.load_store_other; eauto.
-          left. intros Hbb. subst.
-          exploit Genv.find_symbol_injective. apply H2. apply H.
-          intros. easy.
-          intros ofs Hofs. eapply Mem.perm_store_1; eauto.
-        + destruct H4. econstructor; eauto.
-          erewrite Mem.load_store_other; eauto.
-          left. intros Hbb. subst.
-          exploit Genv.find_symbol_injective. apply H3. apply H.
-          intros. easy.
-          intros ofs Hofs. eapply Mem.perm_store_1; eauto.
-        + econstructor; eauto. intros ix.
-          * unfold update in *. destruct Nat.eq_dec.
-            -- subst. exists c_v. split; auto.
-               erewrite Mem.load_store_same; eauto.
-               f_equal.
-               eapply SimplLocalsproof.val_casted_load_result.
-               eapply val_is_int; eauto. reflexivity.
-            -- edestruct (H0 ix) as (vx & Hvx & Hrv).
-               exists vx; split; auto.
-               erewrite Mem.load_store_other; eauto. right.
-               apply not_eq in n. destruct n.
-               ++ right. apply inj_lt in H3. cbn [size_chunk]. lia.
-               ++ left. apply inj_lt in H3. cbn [size_chunk]. lia.
-          * intros ofs Hofs. eapply Mem.perm_store_1; eauto.
-        (* + erewrite Mem.nextblock_store; eauto. *)
+        apply Hrho. constructor.
+        (* temporal conditions *)
+        - apply Mem.unchanged_on_refl.
+        - eapply Mem.store_unchanged_on. exact Hm'.
+          intros ofs Hofs [A B]. apply B.
+          cbn. apply Exists_cons_tl.
+          apply Exists_cons_tl. apply Exists_cons_hd.
+          split. eassumption.
+          replace (size_chunk Mint32) with 4 in * by reflexivity.
+          unfold Nz. lia.
+        (* match return value *)
+        - constructor.
+        (* match return state *)
+        - constructor. 2: repeat apply conj.
+          (* memory extension *)
+          + eapply Mem.store_outside_extends; eauto.
+            intros. apply (Hperm b0 ofs').
+            cbn. apply Exists_cons_tl.
+            apply Exists_cons_tl. apply Exists_cons_hd.
+            split. eassumption.
+            replace (size_chunk Mint32) with 4 in * by reflexivity.
+            unfold Nz. lia.
+            eauto with mem.
+          (* permission *)
+          + apply Hperm.
+          (* defined *)
+          + admit.
+          (* rho relation *)
+          + constructor.
+            * destruct H2. econstructor; eauto.
+              erewrite Mem.load_store_other; eauto.
+              left. intros Hbb. subst.
+              exploit Genv.find_symbol_injective. apply H2. apply H.
+              intros. easy.
+              intros ofs Hofs. eapply Mem.perm_store_1; eauto.
+            * destruct H4. econstructor; eauto.
+              erewrite Mem.load_store_other; eauto.
+              left. intros Hbb. subst.
+              exploit Genv.find_symbol_injective. apply H3. apply H.
+              intros. easy.
+              intros ofs Hofs. eapply Mem.perm_store_1; eauto.
+            * econstructor; eauto. intros ix.
+              -- unfold update in *. destruct Nat.eq_dec.
+                 ++ subst. exists c_v. split; auto.
+                    erewrite Mem.load_store_same; eauto.
+                    f_equal.
+                    eapply SimplLocalsproof.val_casted_load_result.
+                    eapply val_is_int; eauto. reflexivity.
+                 ++ intros Hix. edestruct (H0 _ Hix) as (vx & Hvx & Hrv).
+                    exists vx; split; auto.
+                    erewrite Mem.load_store_other; eauto. right.
+                    apply not_eq in n. destruct n.
+                 ** right. apply inj_lt in H3. cbn [size_chunk]. lia.
+                 ** left. apply inj_lt in H3. cbn [size_chunk]. lia.
+              -- intros ofs Hofs. eapply Mem.perm_store_1; eauto.
       }
       fcd_simpl. inf_intro [ n Hx ]. inv Hx.
       fcd_simpl. sup_mor. apply (fsup_at tt).
@@ -394,6 +389,10 @@ Section RB.
       fcd_simpl. reflexivity.
     (* get *)
     - rename H10 into Hb. rename H12 into Hnb.
+      replace vf' with (Vptr b zero).
+      2: inv Hvinj; inv H1; reflexivity.
+      replace args' with ([Vint (Int.repr (Z.of_nat i2))]).
+      2: { inv Hargs. inv H3. inv H1. reflexivity. }
       apply assert_l. intros Hi.
       setoid_rewrite sup_fsup. sup_mor.
       (* initial_state *)
@@ -405,7 +404,7 @@ Section RB.
       rewrite lts_spec_step. sup_mor. apply join_l. apply join_l.
       (* internal steps *)
       inv HRst. inv H5. rename mm into m.
-      edestruct (H0 i2) as (vx & Hvx & Hvr).
+      edestruct (H0 _ Hi) as (vx & Hvx & Hvr).
       sup_mor. eapply fsup_at.
       {
         cbn. crush_star.
@@ -428,8 +427,14 @@ Section RB.
       fcd_simpl. sup_mor.
       eapply (fsup_at (vx, (m, (f, c1, c2)))).
       {
-        apply Hrho. subst R1. cbn. repeat apply conj; eauto.
-        constructor; eauto. econstructor; eauto.
+        apply Hrho. constructor.
+        (* temporal conditions *)
+        - apply Mem.unchanged_on_refl.
+        - apply Mem.unchanged_on_refl.
+        (* match return value *)
+        - reflexivity.
+        - constructor; eauto. repeat apply conj; eauto.
+          constructor; eauto. econstructor; eauto.
       }
       fcd_simpl. inf_intro [x Hx]. inv Hx.
       fcd_simpl. sup_mor. eapply (fsup_at (f i2)).
@@ -437,6 +442,9 @@ Section RB.
       fcd_simpl. reflexivity.
     (* inc1 *)
     - rename H10 into Hb. rename H11 into Hnb.
+      replace vf' with (Vptr b zero).
+      2: inv Hvinj; inv H1; reflexivity.
+      inv Hargs.
       setoid_rewrite sup_fsup.
       (* initial_state *)
       sup_mor. eapply fsup_at.
@@ -476,45 +484,53 @@ Section RB.
       fcd_simpl. sup_mor.  eapply (fsup_at (Vint i2, m'')).
       { apply HRc. reflexivity. }
       fcd_simpl. sup_mor.
-      eapply (fsup_at (Vint i2, (mm, (f, (S c1 mod CAL.N)%nat, c2)))).
+      eapply (fsup_at (Vint i2, (mm, (f, (S c1 mod BQ.N)%nat, c2)))).
       {
-        apply Hrho. subst R1. cbn. repeat apply conj; eauto. 2: constructor.
-        + assert (Hp: forall ofs', Mem.perm mm b0 ofs' Cur Readable ->
+        apply Hrho. constructor.
+        (* temporal conditions *)
+        - apply Mem.unchanged_on_refl.
+        - admit.
+        (* match return value *)
+        - constructor.
+        (* match state *)
+        - constructor. 2: repeat apply conj; eauto.
+          (* memory extension *)
+          + assert (Hp: forall ofs', Mem.perm mm b0 ofs' Cur Readable ->
                               0 <= ofs' < 0 + size_chunk Mint32 -> False).
-          { intros. unfold AbstractStateRel.no_perm_on in Hperm.
-            apply (Hperm b0 ofs').
-            unfold KRel.blocks. exists cnt1_id. split; auto.
-            apply Mem.perm_cur_max.
-            eapply Mem.perm_implies; eauto. apply perm_any_N. }
-          eapply Mem.store_outside_extends; [ | eauto | eauto ].
-          eapply Mem.store_outside_extends; eauto.
-        + econstructor; eauto.
-          * erewrite Mem.load_store_same; eauto.
-          * cbn. constructor.
-            apply cnt_inc_simp; assumption.
-          * apply Nat.mod_upper_bound. lia.
-          * intros ofs Hofs. eapply Mem.perm_store_1; eauto.
-            eapply Mem.perm_store_1; eauto.
-        + inv H4. econstructor; eauto.
-          * assert (b1 <> b0).
-            { intros <-. exploit Genv.find_symbol_injective.
-              apply H. apply H1. easy. }
-            erewrite Mem.load_store_other. 2: apply Hm''. 2: left; auto.
-            erewrite Mem.load_store_other; eauto.
-          * intros ofs Hofs. eapply Mem.perm_store_1; eauto.
-            eapply Mem.perm_store_1; eauto.
-        + inv H5. assert (b0 <> b1).
-          { intros <-. exploit Genv.find_symbol_injective.
-            apply H. apply H1. easy. }
-          econstructor; eauto.
-          * intros ix. edestruct (H7 ix) as (vx & Hvx & Hrx).
-            exists vx. split; eauto.
-            erewrite Mem.load_store_other. 2: apply Hm''. 2: left; auto.
-            erewrite Mem.load_store_other; eauto.
-          * intros ofs Hofs. eapply Mem.perm_store_1; eauto.
-            eapply Mem.perm_store_1; eauto.
-        (* + erewrite Mem.nextblock_store. 2: apply Hm''. *)
-        (*   erewrite Mem.nextblock_store; eauto. *)
+            { intros. apply (Hperm b0 ofs').
+              apply Exists_exists.
+              eexists (cnt1_id, _). split; auto.
+              cbn. now left. cbn. eauto. eauto with mem. }
+            eapply Mem.store_outside_extends; [ | eauto | eauto ].
+            eapply Mem.store_outside_extends; eauto.
+          (* defined *)
+          + admit.
+          + constructor.
+            * econstructor; eauto.
+              -- erewrite Mem.load_store_same; eauto.
+              -- cbn. constructor.
+                 apply cnt_inc_simp; assumption.
+              -- apply Nat.mod_upper_bound. lia.
+              -- intros ofs Hofs. eapply Mem.perm_store_1; eauto.
+                 eapply Mem.perm_store_1; eauto.
+            * inv H4. econstructor; eauto.
+              -- assert (b1 <> b0).
+                 { intros <-. exploit Genv.find_symbol_injective.
+                   apply H. apply H1. easy. }
+                 erewrite Mem.load_store_other. 2: apply Hm''. 2: left; auto.
+                 erewrite Mem.load_store_other; eauto.
+              -- intros ofs Hofs. eapply Mem.perm_store_1; eauto.
+                 eapply Mem.perm_store_1; eauto.
+            * inv H5. assert (b0 <> b1).
+              { intros <-. exploit Genv.find_symbol_injective.
+                apply H. apply H1. easy. }
+              econstructor; eauto.
+              -- intros ix Hix. edestruct (H7 _ Hix) as (vx & Hvx & Hrx).
+                 exists vx. split; eauto.
+                 erewrite Mem.load_store_other. 2: apply Hm''. 2: left; auto.
+                 erewrite Mem.load_store_other; eauto.
+              -- intros ofs Hofs. eapply Mem.perm_store_1; eauto.
+                 eapply Mem.perm_store_1; eauto.
       }
       fcd_simpl. inf_intro [x Hx]. inv Hx.
       fcd_simpl. sup_mor. eapply (fsup_at c1).
@@ -522,6 +538,9 @@ Section RB.
       fcd_simpl. reflexivity.
     (* inc2 *)
     - rename H10 into Hb. rename H11 into Hnb.
+      replace vf' with (Vptr b zero).
+      2: inv Hvinj; inv H1; reflexivity.
+      inv Hargs.
       setoid_rewrite sup_fsup.
       (* initial_state *)
       sup_mor. eapply fsup_at.
@@ -561,51 +580,59 @@ Section RB.
       fcd_simpl. sup_mor.  eapply (fsup_at (Vint i2, m'')).
       { apply HRc. reflexivity. }
       fcd_simpl. sup_mor.
-      eapply (fsup_at (Vint i2, (mm, (f, c1, (S c2 mod CAL.N)%nat)))).
+      eapply (fsup_at (Vint i2, (mm, (f, c1, (S c2 mod BQ.N)%nat)))).
       {
-        apply Hrho. subst R1. cbn. repeat apply conj; eauto. 2: constructor.
-        + assert (Hp: forall ofs', Mem.perm mm b0 ofs' Cur Readable ->
+        apply Hrho. constructor.
+        (* temporal conditions *)
+        - apply Mem.unchanged_on_refl.
+        - admit.
+        (* match return value *)
+        - constructor.
+        (* match state *)
+        - constructor. 2: repeat apply conj; eauto.
+          (* memory extension *)
+          + assert (Hp: forall ofs', Mem.perm mm b0 ofs' Cur Readable ->
                               0 <= ofs' < 0 + size_chunk Mint32 -> False).
-          { intros. unfold AbstractStateRel.no_perm_on in Hperm.
-            apply (Hperm b0 ofs').
-            unfold KRel.blocks. exists cnt2_id. split; auto.
-            apply Mem.perm_cur_max.
-            eapply Mem.perm_implies; eauto. apply perm_any_N. }
-          eapply Mem.store_outside_extends; [ | eauto | eauto ].
-          eapply Mem.store_outside_extends; eauto.
-        + inv H2. econstructor; eauto.
-          * assert (b1 <> b0).
-            { intros <-. exploit Genv.find_symbol_injective.
-              apply H. apply H1. easy. }
-            erewrite Mem.load_store_other. 2: apply Hm''. 2: left; auto.
-            erewrite Mem.load_store_other; eauto.
-          * intros ofs Hofs. eapply Mem.perm_store_1; eauto.
-            eapply Mem.perm_store_1; eauto.
-        + econstructor; eauto.
-          * erewrite Mem.load_store_same; eauto.
-          * cbn. constructor.
-            apply cnt_inc_simp; assumption.
-          * apply Nat.mod_upper_bound. lia.
-          * intros ofs Hofs. eapply Mem.perm_store_1; eauto.
-            eapply Mem.perm_store_1; eauto.
-        + inv H5. assert (b0 <> b1).
-          { intros <-. exploit Genv.find_symbol_injective.
-            apply H. apply H1. easy. }
-          econstructor; eauto.
-          * intros ix. edestruct (H7 ix) as (vx & Hvx & Hrx).
-            exists vx. split; eauto.
-            erewrite Mem.load_store_other. 2: apply Hm''. 2: left; auto.
-            erewrite Mem.load_store_other; eauto.
-          * intros ofs Hofs. eapply Mem.perm_store_1; eauto.
-            eapply Mem.perm_store_1; eauto.
-        (* + erewrite Mem.nextblock_store. 2: apply Hm''. *)
-        (*   erewrite Mem.nextblock_store; eauto. *)
+            { intros. apply (Hperm b0 ofs').
+              apply Exists_exists.
+              eexists (cnt2_id, _). split; auto.
+              cbn. now right; left. cbn. eauto. eauto with mem. }
+            eapply Mem.store_outside_extends; [ | eauto | eauto ].
+            eapply Mem.store_outside_extends; eauto.
+          (* defined *)
+          + admit.
+          + constructor.
+            * inv H2. econstructor; eauto.
+              -- assert (b1 <> b0).
+                 { intros <-. exploit Genv.find_symbol_injective.
+                   apply H. apply H1. easy. }
+                 erewrite Mem.load_store_other. 2: apply Hm''. 2: left; auto.
+                 erewrite Mem.load_store_other; eauto.
+              -- intros ofs Hofs. eapply Mem.perm_store_1; eauto.
+                 eapply Mem.perm_store_1; eauto.
+            * econstructor; eauto.
+              -- erewrite Mem.load_store_same; eauto.
+              -- cbn. constructor.
+                 apply cnt_inc_simp; assumption.
+              -- apply Nat.mod_upper_bound. lia.
+              -- intros ofs Hofs. eapply Mem.perm_store_1; eauto.
+                 eapply Mem.perm_store_1; eauto.
+            * inv H5. assert (b0 <> b1).
+              { intros <-. exploit Genv.find_symbol_injective.
+                apply H. apply H1. easy. }
+              econstructor; eauto.
+              -- intros ix Hix. edestruct (H7 _ Hix) as (vx & Hvx & Hrx).
+                 exists vx. split; eauto.
+                 erewrite Mem.load_store_other. 2: apply Hm''. 2: left; auto.
+                 erewrite Mem.load_store_other; eauto.
+              -- intros ofs Hofs. eapply Mem.perm_store_1; eauto.
+                 eapply Mem.perm_store_1; eauto.
       }
       fcd_simpl. inf_intro [x Hx]. inv Hx.
       fcd_simpl. sup_mor. eapply (fsup_at c2).
       { apply Hsub. constructor. constructor. eauto. }
       fcd_simpl. reflexivity.
-  Qed.
+  Admitted.
 
 End RB.
 
@@ -616,24 +643,21 @@ Program Definition empty_rc : esig_rc 0 :=
   {|
     esig_refconv := empty_rc_rel;
   |}.
-Next Obligation. rc_inversion H. Qed.
 
 Program Definition empty_rho : rho_rel unit :=
   {|
     rho_pred se tt m := True;
-    rho_footprint i := False;
+    rho_footprint := nil;
   |}.
-Next Obligation.
-  unfold KRel.blocks in H0.
-  destruct H0 as (? & [] & ?).
-Qed.
+Next Obligation. inv H0. Qed.
+Next Obligation. inv H0. Qed.
 
 Unset Asymmetric Patterns.
 
 Definition dummy_state {E} : E ~> E # unit :=
-  fun _ '(esig_tens_intro m t) =>
+  fun _ '(etens_intro m t) =>
     match t with
-    | state_event tt => ISpec.int m >>= (fun n => ret (n ,tt))
+    | est_intro tt => ISpec.int m >>= (fun n => ret (n ,tt))
     end.
 
 (*
@@ -700,7 +724,7 @@ Section BQ.
   Lemma bq_code_correct:
     dummy_state @ M_bq [=
       slift (right_arrow bq_rc) @ h
-      @ (right_arrow (rho_with_se empty_rho))
+      @ (right_arrow (rho_rc empty_rho))
       @ right_arrow c_rc
       @ ang_lts_spec (semantics2 bq_program)
       @ left_arrow c_rc
@@ -739,12 +763,17 @@ Section BQ.
     unfold compose. cbn.
     unfold assume. inf_intro Hse. intm.
     rc_elim (inv) Hc. depsubst. inv H. inv H0. rename Hsub into HRc.
-    rc_elim (inv) Hrho. depsubst. rename Hsub into HRho. inv H1.
-    rename H into Hm. destruct H0 as [Hx Hperm]. inv Hx.
+    rc_elim (inv) Hrho. depsubst. rename Hsub into HRho.
+    rename H12 into Hvdef. rename H13 into Hvinj. rename H14 into Hargs.
+    inv H6. rename H into Hm. destruct H0 as [Hperm [Hdef Hx]]. inv Hx.
     rename se' into se.
     rc_elim (inv) Hr; unfold mem in *; depsubst; clear_hyp.
     (* enq *)
     - rename H10 into Hb. rename H11 into Hv.
+      replace vf' with (Vptr b zero).
+      2: inv Hvinj; inv H1; reflexivity.
+      replace args' with [c_v].
+      2: admit.
       edestruct inc2_block as (inc2b & Hb1 & Hb2); eauto.
       edestruct set_block as (setb & Hb3 & Hb4); eauto.
       setoid_rewrite sup_fsup.
@@ -827,13 +856,20 @@ Section BQ.
       fcd_simpl. sup_mor. eapply (fsup_at (_, _)).
       { cbn. apply HRc. subst R0. reflexivity. }
       fcd_simpl. sup_mor. eapply (fsup_at (_, (_, tt))).
-      { apply HRho. subst R1. cbn. repeat apply conj; eauto. }
+      { apply HRho. constructor.
+        1-2: eapply Mem.unchanged_on_refl. reflexivity.
+        constructor; eauto.
+        repeat apply conj; eauto.
+        constructor. }
       fcd_simpl. inf_intro [ x Hx ]. inv Hx.
       fcd_simpl. sup_mor. eapply (fsup_at tt).
       apply Hsub. constructor. constructor.
       fcd_simpl. unfold ret. reflexivity.
     (* deq *)
     - rename H10 into Hb.
+      replace vf' with (Vptr b zero).
+      2: inv Hvinj; inv H1; reflexivity.
+      inv Hargs.
       edestruct inc1_block as (inc1b & Hb1 & Hb2); eauto.
       edestruct get_block as (getb & Hb3 & Hb4); eauto.
       (* initial_state *)
@@ -898,8 +934,8 @@ Section BQ.
       inf_intro [ [rv m''] Hrm ]. inv Hrm.
       fcd_simpl. apply join_r.
       inf_intro [ rc Hrc ]. subst. fcd_simpl.
-      replace (FCD.emb (pcons (CAL.get n) v (pret (v, tt))))
-        with (FCD.ext (fun s => FCD.emb (pcons (CAL.get n) v s)) (ret (v, tt))).
+      replace (FCD.emb (pcons (BQ.get n) v (pret (v, tt))))
+        with (FCD.ext (fun s => FCD.emb (pcons (BQ.get n) v s)) (ret (v, tt))).
       2: { setoid_rewrite FCD.ext_ana. reflexivity. }
       rstep. sup_mor. eapply fsup_at.
       { constructor. }
@@ -913,12 +949,16 @@ Section BQ.
       fcd_simpl. sup_mor. eapply (fsup_at (_, _)).
       { cbn. apply HRc.  subst R0. reflexivity. }
       fcd_simpl. sup_mor. eapply (fsup_at (_, (_, tt))).
-      { apply HRho. subst R1. cbn. repeat apply conj; eauto. }
+      { apply HRho. constructor.
+        1-2: eapply Mem.unchanged_on_refl. reflexivity.
+        constructor; eauto.
+        repeat apply conj; eauto.
+        constructor. }
       fcd_simpl. inf_intro [x Hx]. inv Hx.
       fcd_simpl. sup_mor. eapply (fsup_at v).
       { apply Hsub. constructor. eauto. }
       fcd_simpl. reflexivity.
-  Qed.
+  Admitted.
 
 End BQ.
 
@@ -926,7 +966,7 @@ Require Composition.
 Transparent CModule.semantics.
 
 Lemma singleton_module_ref p:
-  ang_lts_spec (semantics2 p) [= ang_lts_spec (CModule.semantics [p] (erase_program p)).
+  ang_lts_spec (semantics2 p) [= ang_lts_spec (CModule.semantics (CModule.cmod_of_program p)).
 Proof.
   pose proof @Composition.hcomp_singleton_fsim.
   apply ang_fsim_embed_cc_id.
@@ -958,8 +998,7 @@ Program Definition rb_correct: strategy_clight L_rb :=
     rho := rho_rb;
     r1 := empty_rc;
     r2 := rb_rc;
-    M := [ rb_program ];
-    sk := AST.erase_program rb_program;
+    M := CModule.cmod_of_program rb_program;
   |}.
 Local Obligation Tactic := idtac.
 Next Obligation.
@@ -983,8 +1022,7 @@ Program Definition bq_correct : strategy_clight (dummy_state @ M_bq) :=
     rho := empty_rho;
     r1 := rb_rc;
     r2 := bq_rc;
-    M := [ bq_program ];
-    sk := AST.erase_program bq_program;
+    M := CModule.cmod_of_program bq_program;
   |}.
 Next Obligation.
   rewrite bq_code_correct. cbn -[left_arrow right_arrow].
