cal/CompCertCAL.v
@@ -1,0 +1,664 @@
+From Coq Require Import
+     List Lia.
+From models Require Import
+     IntSpec.
+From cal Require Import
+     RefConv CompCertIntSpec
+     IntSpecCAL.
+From lattices Require Import
+     Upset Downset FCD.
+From structures Require Import
+     Effects Lattice.
+From compcert Require Import
+     Coqlib
+     AST Values Memory
+     Globalenvs
+     LanguageInterface
+     Smallstep.
+From compcertox Require Import
+     Lifting CModule AbRel.
+Import ListNotations ISpec.
+
+Unset Asymmetric Patterns.
+
+(** * CompCert Layers *)
+
+(** The language interface "C simple" which does not include the memory *)
+Inductive c_esig : esig :=
+| c_event : val -> signature -> list val -> Genv.symtbl -> c_esig val.
+
+Inductive c_rc: rc_rel (c_esig # mem) li_c :=
+| c_rc_intro vf sg args e_c e_s m se:
+  let R := (fun '(r, m) c_r => c_r = cr r m) in
+  e_c = c_event vf sg args se -> e_s = est_intro m ->
+  c_rc _ (etens_intro e_c e_s) _ (eli_intro (cq vf sg args m) se) R.
+
+Close Scope Z_scope.
+Record clight_layer {S1 S2} (L1: 0 ~> (li_c @ S1)%li) (L2: 0 ~> (li_c @ S2)%li) :=
+  {
+    clight_impl: cmodule;
+    clight_rel: abrel S2 S1;
+
+    clight_layer_ref:
+      let MS := ang_lts_spec (((semantics clight_impl) @ S1)%lts)
+      in L2 [= right_arrow (cc_rc clight_rel) @ MS @ L1;
+  }.
+Arguments clight_impl {_ _ _ _}.
+Arguments clight_rel {_ _ _ _}.
+Arguments clight_layer_ref {_ _ _ _}.
+
+(*
+Section CAT_APP.
+  Context {M N sk1 sk2} `{!CategoricalComp.CategoricalLinkable (semantics M sk1) (semantics N sk2)}.
+
+  Lemma cmodule_categorical_comp_simulation sk:
+    forward_simulation
+      1 1
+      (CategoricalComp.comp_semantics' (semantics M sk1) (semantics N sk2) sk)
+      (semantics (M ++ N) sk).
+  Proof.
+    etransitivity.
+    2: { apply cmodule_categorical_comp_simulation.
+         unfold CategoricalComp.CategoricalLinkable in *.
+         cbn in *. apply H. }
+    etransitivity.
+    2: { apply lift_comp_component. }
+    instantiate (1 := sk2).
+    instantiate (1 := sk1).
+    unfold skel_extend. reflexivity.
+  Qed.
+
+  Lemma cmodule_categorical_comp_simulation_lifted sk S:
+    forward_simulation
+      1 1
+      (CategoricalComp.comp_semantics' (semantics M sk1 @ S) (semantics N sk2 @ S) sk)
+      (semantics (M ++ N) sk @ S).
+  Proof.
+    pose proof (cmodule_categorical_comp_simulation sk) as HX.
+    eapply (@lifting_simulation S) in HX.
+    etransitivity. 2: apply HX.
+    apply lift_categorical_comp2.
+  Qed.
+End CAT_APP.
+ *)
+
+Lemma cmodule_rel {S1 S2} M (R: abrel _ _):
+  ang_lts_spec (semantics M @ S2) @ right_arrow (cc_rc R) [=
+    right_arrow (cc_rc R) @ ang_lts_spec (semantics M @ S1).
+Proof.
+  pose proof (cmodule_abrel R M) as H.
+  eapply ang_fsim_embed in H. rewrite H.
+  cbn -[LatticeProduct.poset_prod].
+  rewrite !compose_assoc.
+  rewrite @rc_adj_epsilon. rewrite compose_unit_r. reflexivity.
+Qed.
+
+(** ** Composition *)
+Section COMP.
+
+  Context {Ks Kn Kf}
+          (Ls: 0 ~> (li_c @ Ks)%li)
+          (Ln: 0 ~> (li_c @ Kn)%li)
+          (Lf: 0 ~> (li_c @ Kf)%li)
+          (C1: clight_layer Ls Ln) (C2: clight_layer Ln Lf).
+  Context C (HC: cmod_app (clight_impl C2) (clight_impl C1) = Some C).
+  Context (HR: disjoint_abrel (clight_rel C2) (clight_rel C1)).
+  Context (Hcomp: CategoricalComp.CategoricalLinkable
+                    (semantics (clight_impl C2))
+                    (semantics (clight_impl C1))).
+
+  Local Obligation Tactic := idtac.
+
+  (* Embedded version of layer_vcomp] from Compsition.v *)
+  Program Definition clight_layer_compose: clight_layer Ls Lf :=
+    {|
+      clight_impl := C;
+      clight_rel := abrel_comp (clight_rel C2) (clight_rel C1);
+    |}.
+  Next Obligation.
+    destruct C1 as [M1 R1 Hsim1].
+    destruct C2 as [M2 R2 Hsim2].
+    Local Opaque LatticeProduct.poset_prod.
+    cbn -[semantics right_arrow] in *. etransitivity.
+    apply Hsim2. clear Hsim2.
+    rewrite Hsim1. clear Hsim1.
+    rewrite <- (compose_assoc _ (right_arrow (cc_rc R1)) _).
+    rewrite cmodule_rel; eauto. rewrite compose_assoc.
+    rewrite <- (compose_assoc _ (right_arrow R1) _).
+    apply compose_proper_ref.
+    {
+      rewrite right_arrow_compose. apply right_arrow_monotonic.
+      unfold cc_refconv.        (* we could not make it a coercion *)
+      rewrite <- cc_rc_compose. apply cc_rc_ref.
+      apply krel_comp_ref. exact HR.
+    }
+    rewrite <- compose_assoc.
+    apply compose_proper_ref. 2: reflexivity.
+    erewrite (comp_embed (semantics M2 @ Ks)%lts (semantics M1 @ Ks)%lts).
+    2: { unfold CategoricalComp.comp_semantics. cbn.
+         erewrite cmod_app_skel. reflexivity. apply HC. }
+    apply ang_fsim_embed_cc_id.
+    etransitivity. apply lift_categorical_comp2.
+    apply lifting_simulation.
+    apply cmodule_categorical_comp_simulation; eauto.
+  Qed.
+
+End COMP.
+
+(** * Connection between the Strategy World and the CompCert World *)
+
+Require Import Events.
+
+Record rho_rel (U: Type) :=
+  {
+    rho_pred (se: Genv.symtbl) :> U -> mem -> Prop;
+    rho_footprint : list (ident * Z);
+
+    rho_ext (se: Genv.symtbl) : mem * U -> mem -> Prop :=
+      fun '(m1, u) m2 =>
+        Mem.extends m1 m2
+        /\ (forall b ofs, locsp se rho_footprint b ofs -> loc_out_of_bounds m1 b ofs)
+        /\ defined_on (fun b ofs => Mem.perm m2 b ofs Max Nonempty
+                                /\ loc_out_of_bounds m1 b ofs) m2
+        /\ rho_pred se u m2;
+
+    rho_invar : forall se u m m',
+      rho_pred se u m ->
+      Mem.unchanged_on (locsp se rho_footprint) m m' ->
+      rho_pred se u m';
+    rho_valid : forall se u m b ofs,
+      rho_pred se u m -> (locsp se rho_footprint) b ofs -> Mem.valid_block m b;
+    rho_perm : forall se u m b ofs,
+      rho_pred se u m -> (locsp se rho_footprint) b ofs -> Mem.perm m b ofs Max Nonempty;
+  }.
+
+Arguments rho_footprint {_} _.
+Arguments rho_ext {_} _.
+
+Inductive rho_rc_reply {U:Type} (rho: rho_rel U) se m1 m2 : val * (mem * U) -> val * mem -> Prop :=
+| rho_rc_reply_intro r1 r2 u n1 n2
+   (ACCMS: Mem.unchanged_on (loc_out_of_bounds m1) m1 n1)
+   (ACCMF: Mem.unchanged_on (fun b ofs => loc_out_of_bounds m1 b ofs /\
+                                         ~ locsp se (rho_footprint rho) b ofs) m2 n2)
+   (RETINJ: Val.inject inject_id r1 r2)
+   (ABS: rho_ext rho se (n1, u) n2):
+  rho_rc_reply rho se m1 m2 (r1, (n1, u)) (r2, n2).
+
+Inductive rho_rc {U} (rho: rho_rel U): rc_rel (c_esig # (mem * U)) (c_esig # mem) :=
+| rho_rc_intro vf1 vf2 sg vargs1 vargs2 se u m1 m2:
+  rho_ext rho se (m1, u) m2 ->
+  vf1 <> Vundef ->
+  Val.inject inject_id vf1 vf2 ->
+  Val.inject_list inject_id vargs1 vargs2 ->
+  rho_rc rho _ (c_event vf1 sg vargs1 se # (m1, u)) _ (c_event vf2 sg vargs2 se # m2)
+         (rho_rc_reply rho se m1 m2).
+
+Program Definition rho_abrel {S1 S2 U} (R: S2 -> U * S1 -> Prop) (rho: rho_rel U) : abrel S2 S1 :=
+  {|
+    abrel_pred se := fun s2 '(m, s1) => exists u, R s2 (u, s1) /\ rho se u m;
+    abrel_footprint := rho_footprint rho;
+  |}.
+Next Obligation.
+  eexists; split; eauto.
+  eapply rho_invar; eauto.
+Qed.
+Next Obligation.
+  eapply rho_valid; eauto.
+Qed.
+Next Obligation.
+  eapply rho_perm; eauto.
+Qed.
+
+Inductive li_state_rc {li: language_interface} {S: Type}: rc_rel (li # S) (li @ S)%li :=
+| li_state_rc_intro (q: query li) s se:
+  li_state_rc _ (eli_intro q se # s) _ (eli_intro (li:=li@S) (q, s) se) eq.
+
+Definition c_mem_state_rc {S: Type}: rc_rel (c_esig # (mem * S)) (li_c @ S)%li :=
+  rc_compose sig_assoc (rc_compose  (c_rc * rc_id) li_state_rc).
+
+Close Scope Z_scope.
+
+Record esig_rc (E: esig) :=
+  {
+    esig_refconv :> refconv E (c_esig # mem);
+    (*
+    esig_rc_clo :
+      forall ar e R vf1 sg vargs1 m vf2 vargs2 se,
+        esig_refconv ar e _ (c_event vf1 sg vargs1 se # m) R ->
+        Val.inject inject_id vf1 vf2 -> Val.inject_list inject_id vargs1 vargs2 ->
+        esig_refconv ar e _ (c_event vf2 sg vargs2 se # m) R;
+     *)
+  }.
+
+
+Section REL_REF.
+
+  Context {S1 S2 U} (R: S2 -> U * S1 -> Prop) (rho: rho_rel U).
+  Context {E2} (r2: esig_rc E2).
+
+  Definition lhs: (li_c @ S1)%li ~> (li_c @ S2)%li :=
+    left_arrow c_mem_state_rc
+    @@ slift (left_arrow r2)
+    @ right_arrow (rc_id * rel_rc R)
+    @ slift (right_arrow r2)
+    @ h @ h @ h
+    @ slift (right_arrow (rho_rc rho))
+    @@ right_arrow c_mem_state_rc.
+
+  Definition rhs: (li_c @ S1)%li ~> (li_c @ S2)%li := right_arrow (rho_abrel R rho).
+
+  Lemma rel_ref: lhs [= rhs.
+  Proof.
+    unfold lhs, rhs. cbn. intros ? [ [ q s2 ] ].
+    cbn. unfold rc_adj_right at 8.
+    apply inf_iff. intros ?. apply inf_iff. intros qs1.
+    apply inf_iff. intros (Rx & HR). cbn.
+    destruct HR as (Rx' & Hrel & Hsub).
+    inversion Hrel. cbn in *. depsubst. clear Hrel H4 H1.
+    rename H7 into Hq. destruct q2 as [ q1 s1 ].
+    inv Hq. inv H5. inv ABS. rename x into u. destruct H as [ HR Hrho ].
+    rename se2 into se.
+
+    match goal with
+    | |- context [ _ @ ?f ] => set (f1 := f)
+    end.
+    unfold compose. unfold rc_adj_left.
+    sup_intro ?. sup_intro m. sup_intro (Ra & HRa).
+    rc_elim (inv) HRa. depsubst.
+    rc_elim (inv) H4. depsubst. clear_hyp.
+    rc_elim (inv) H5. depsubst.
+    rc_elim (inv) H5. cbn in *. depsubst. clear_hyp.
+    rc_elim (inv) H4. depsubst. clear_hyp.
+    rc_elim (inv) H2. depsubst. clear_hyp. inv H4.
+    (* rc_id is tricky *)
+    rc_inversion H13. simple inversion Hrel. depsubst. clear_hyp. inv H7.
+    clear Hrel. intm. unfold f1 at 2.
+
+    match goal with
+    | |- context [ _ @ ?f' ] => set (f2 := f')
+    end.
+    unfold compose. unfold rc_adj_right.
+    inf_mor. eapply inf_at.
+    inf_mor. eapply (inf_at (c_event vfs sg vargss se # s0 # s2)).
+    inf_mor. eapply finf_at. rc_econstructor.
+    intm. unfold f2 at 2.
+
+    match goal with
+    | |- context [ _ @ ?f' ] => set (f3 := f')
+    end.
+    unfold compose. cbn. unfold rc_adj_left.
+    sup_intro ?. sup_intro e2. sup_intro [Rr2 Hr2].
+    intm. unfold f3 at 2.
+
+    match goal with
+    | |- context [ _ @ ?f' ] => set (f4 := f')
+    end.
+    unfold compose. unfold rc_adj_right.
+    inf_mor. eapply inf_at.
+    inf_mor. eapply (inf_at (e2 # (u, s1))).
+    inf_mor. eapply finf_at.
+    { rc_econstructor; rc_econstructor. easy. }
+    intm. unfold f4 at 2.
+
+    match goal with
+    | |- context [ _ @ ?f' ] => set (f5 := f')
+    end.
+    unfold compose. cbn. unfold rc_adj_right.
+    inf_mor. eapply inf_at.
+    inf_mor. eapply (inf_at (c_event vfs sg vargss se # s0)).
+    inf_mor. eapply finf_at. instantiate (1 := Rr2).
+    exact Hr2. intm. unfold f5 at 2.
+
+    match goal with
+    | |- context [ _ @ ?f' ] => set (f6 := f')
+    end.
+    unfold compose. unfold rc_adj_left.
+    sup_intro ?. sup_intro m. sup_intro [ Rb Hrb ].
+    destruct m. destruct e. destruct p. destruct p.
+    rc_elim (inv) Hrb. depsubst. clear_hyp.
+    intm. unfold f6 at 2.
+
+    match goal with
+    | |- context [ _ @ ?f' ] => set (f7 := f')
+    end.
+    unfold compose. unfold rc_adj_right.
+    inf_mor. eapply inf_at.
+    inf_mor. eapply (inf_at (c_event vfs sg vargss se # (s0, u, s1))).
+    inf_mor. eapply finf_at.
+    { rc_econstructor; rc_econstructor. constructor. }
+    intm. unfold f7 at 2.
+
+    match goal with
+    | |- context [ _ @ ?f' ] => set (f8 := f')
+    end.
+    unfold compose. unfold rc_adj_right.
+    inf_mor. eapply inf_at.
+    inf_mor. eapply (inf_at (c_event vfs sg vargss se # (s0, u) # s1)).
+    inf_mor. eapply finf_at. rc_econstructor.
+    intm. unfold f8 at 2.
+
+    match goal with
+    | |- context [ _ @ ?f' ] => set (f9 := f')
+    end.
+    unfold compose. cbn. unfold rc_adj_right.
+    inf_mor. eapply inf_at.
+    inf_mor. eapply (inf_at (c_event vff sg vargsf se # mf)).
+    inf_mor. eapply finf_at.
+    { rc_econstructor. 2-4: eauto.
+      constructor. auto. split; auto. }
+    intm. unfold f9 at 2.
+
+    unfold compose. unfold rc_adj_left.
+    sup_intro ?. sup_intro m. sup_intro [ Rc Hrc ].
+    destruct m. destruct e. destruct p.
+    rc_elim (inv) Hrc. depsubst. clear_hyp. intm.
+
+    unfold rc_adj_right at 2.
+    inf_mor. eapply inf_at.
+    inf_mor. eapply (inf_at ((eli_intro (li:=li_c@S1)(cq vff sg vargsf mf ,s1) se))).
+    inf_mor. eapply finf_at.
+    { repeat rc_econstructor; reflexivity. }
+    intm.
+
+    apply int_ref. intros [cr s1'].
+    sup_intro (x & Hx).
+    destruct cr as [ r m' ]. destruct x. destruct p.
+    inv Hx. destruct H. inv H. inv H0. destruct H.
+    subst x. destruct H. cbn in *. inv H.
+    fcd_simpl.
+    inf_mor. apply (finf_at (v, m, s1')).
+    apply Hsub8. constructor.
+    fcd_simpl. sup_intro (x & Hx).
+    (* rho_with_se *)
+    destruct x. destruct p. inv Hx.
+    fcd_simpl. sup_intro (x & Hx).
+    (* assoc *)
+    destruct x. destruct p. destruct p. inv Hx.
+    fcd_simpl. sup_intro (x & Hx).
+    (* eq * assoc *)
+    destruct x. destruct p. destruct p. destruct Hx. cbn in *. inv H0.
+    fcd_simpl.
+    inf_mor. apply (finf_at (v0, m0, (u0, s1'))).
+    apply Hsub7. constructor.
+    fcd_simpl. sup_intro (n2 & Hr2').
+    fcd_simpl. sup_intro (x & Hx). destruct x. destruct Hx. cbn in *. subst.
+    fcd_simpl. inf_mor. apply (finf_at (v0, m0)). apply Hr2'.
+    fcd_simpl. sup_intro (x & Hx). destruct x. destruct p. inv Hx.
+    fcd_simpl. inf_mor. apply (finf_at (cr v0 m0, s)).
+    apply Hsub0. eexists; split.
+    apply Hsub1. constructor.
+    apply Hsub2. eexists; split.
+    apply Hsub4. instantiate (1 := (_, _)). split.
+    apply Hsub5. subst R5. cbn. reflexivity.
+    apply Hsub6. cbn. reflexivity.
+    apply Hsub3. reflexivity.
+    fcd_simpl. clear f1 f2 f3 f4 f5 f6 f7 f8 f9.
+    apply (fsup_at (cr v0 m0, s)).
+    apply Hsub.
+    exists (mk_aw se m0 m). split.
+    - constructor; eauto.
+    - constructor; eauto.
+      all: try apply ABS.
+      exists u0. split; eauto. apply ABS.
+    - fcd_simpl. reflexivity.
+  Qed.
+
+End REL_REF.
+
+Section STRATEGY_REF.
+
+  Record strategy_clight {E1 E2 U} (Sigma: E1 ~> E2 # U) :=
+    {
+      rho : rho_rel U;
+      r1 : esig_rc E1;
+      r2 : esig_rc E2;
+      M: cmodule;
+
+      strategy_clight_ref:
+        left_arrow c_rc
+        @ left_arrow (rho_rc rho)
+        @@ slift (left_arrow r2)
+        @ Sigma
+        @ right_arrow r1
+        @ right_arrow c_rc
+        [= ang_lts_spec (semantics M)
+    }.
+
+End STRATEGY_REF.
+
+Lemma lift_lts_ref {liA liB} (L: Smallstep.semantics liA liB) (K: Type):
+  left_arrow li_state_rc @ slift (ang_lts_spec L) @ right_arrow li_state_rc [=
+    ang_lts_spec (L@K)%lts.
+Proof.
+  cbn. intros ? [[qb k] se].
+  unfold rc_adj_left, rc_adj_right, compose. cbn.
+  sup_intro ?. sup_intro [? ? [qb' se'] [k']].
+  sup_intro [Rx HRx]. rc_elim (inv) HRx. depsubst. intm.
+  apply assume_r. intros Hse.
+  unfold assume. inf_mor. apply (inf_at Hse). fcd_simpl.
+  rewrite sup_fsup. sup_intro [si Hsi].
+  rewrite sup_fsup. eapply (fsup_at (si, k)).
+  { constructor; eauto. }
+  sup_intro steps. apply (sup_at steps).
+  clear Hsi. revert si k. induction steps.
+  - intros si k. cbn. repeat sup_mor. reflexivity.
+  - intros si k. Opaque lifted_semantics.
+    cbn. sup_mor. repeat apply join_lub.
+    + apply join_l. apply join_l.
+      sup_intro (st & Hst).
+      eapply (fsup_at (st, k)).
+      { now apply lifting_step_star. }
+      apply IHsteps.
+    + apply join_l. apply join_r.
+      sup_intro (qa & Hq). eapply (fsup_at (qa, k)).
+      { constructor; eauto. }
+      unfold query_int. intm.
+      inf_mor. eapply inf_at.
+      inf_mor. eapply (inf_at (eli_intro (li:=(liA@K)) (qa, k) se)).
+      inf_mor. eapply finf_at.
+      { rc_econstructor. }
+      intm. unfold int at 3 4.
+      sup_intro [[ra k']|].
+      * fcd_simpl. apply join_lub.
+        -- apply (sup_at None). fcd_simpl. reflexivity.
+        -- apply (sup_at (Some (ra, k'))). fcd_simpl.
+           apply join_r. rstep.
+           sup_intro ((ra', k'') & Hr). inv Hr.
+           intm. sup_intro (s' & Hs').
+           eapply (fsup_at (s', k')).
+           { constructor; eauto. }
+           apply IHsteps.
+      * apply (sup_at None). fcd_simpl. reflexivity.
+    + apply join_r. sup_intro (r & Hr).
+      apply (fsup_at (r, k)).
+      { constructor; eauto. }
+      fcd_simpl.
+      inf_mor. eapply (finf_at (_, _)). apply Hsub. reflexivity.
+      fcd_simpl. reflexivity.
+Qed.
+
+Lemma lift_rc_r {E F S} (r: E <=> F):
+  right_arrow (r * rc_id) = slift (S:=S) (right_arrow r).
+Proof.
+  apply antisymmetry; intros ? [? ? m [s]]; cbn; unfold rc_adj_right.
+  - inf_intro ?. inf_intro ?.
+    inf_intro (R & HR).
+    eapply inf_at. eapply inf_at.
+    eapply finf_at.
+    { rc_econstructor; [ eauto | rc_econstructor ]. }
+    intm. unfold int.
+    sup_intro [[n t]|].
+    + fcd_simpl. apply join_lub.
+      * apply (sup_at None). now fcd_simpl.
+      * apply (sup_at (Some (n, t))).
+        fcd_simpl. apply join_r. rstep.
+        sup_intro ((x, t') & Hr). inv Hr.
+        cbn in *. subst.
+        eapply (fsup_at x). eauto. now fcd_simpl.
+    + apply (sup_at None). fcd_simpl. reflexivity.
+  - inf_intro ?. inf_intro ?. inf_intro (R & HR).
+    rc_elim (inv) HR. depsubst. clear_hyp.
+    destruct m2'. destruct H11 as (Rx & (Hx & Hy)).
+    simple inversion Hx. clear Hx. depsubst. clear_hyp. inv H2.
+    eapply inf_at. eapply inf_at.
+    (* fixme *)
+    eapply (inf_at (exist _ _ H6)).
+    intm. unfold int.
+    sup_intro [[n t]|].
+    + fcd_simpl. apply join_lub.
+      * apply (sup_at None). fcd_simpl. reflexivity.
+      * apply (sup_at (Some (n, t))).
+        fcd_simpl. apply join_r. rstep.
+        sup_intro (x & Hr).
+        eapply (fsup_at (x, t)). apply Hsub.
+        split; eauto. now fcd_simpl.
+    + apply (sup_at None). fcd_simpl. reflexivity.
+Qed.
+
+Lemma lift_rc_l S:
+  left_arrow (c_rc * rc_id) = slift (S:=S) (left_arrow c_rc).
+Admitted.
+
+Section COMPILE_LAYER.
+
+  Context {E1 E2 S1 S2 U} (L1: 0 ~> E1 # S1) (L2: 0 ~> E2 # S2)
+          (st_layer: strategy_layer U L1 L2).
+  Context (st_clight: strategy_clight (strategy_impl st_layer)).
+
+  Definition Lc1: 0 ~> (li_c @ S1)%li :=
+    left_arrow c_mem_state_rc @@ slift (left_arrow (r1 _ st_clight)) @ L1.
+
+  Definition Lc2: 0 ~> (li_c @ S2)%li :=
+    left_arrow c_mem_state_rc @@ slift (left_arrow (r2 _ st_clight)) @ L2.
+
+  Local Obligation Tactic := idtac.
+  Local Opaque semantics.
+
+  Program Definition c_layer: clight_layer Lc1 Lc2 :=
+    {|
+      clight_impl := M _ st_clight;
+      clight_rel := (rho_abrel (strategy_rel st_layer) (rho _ st_clight));
+    |}.
+  Next Obligation.
+    unfold Lc1, Lc2.
+    destruct st_clight as [ rho r1 r2 M strategy_clight_ref ].
+    destruct st_layer as [ Sigma R strategy_layer_ref ].
+    Local Opaque LatticeProduct.poset_prod.
+    Local Opaque left_arrow right_arrow.
+    cbn in *.
+    pose proof (rel_ref R rho r2) as H. unfold lhs, rhs in H. cbn in *.
+    rewrite <- H. clear H.
+    rewrite <- lift_lts_ref.
+    rewrite strategy_layer_ref. clear strategy_layer_ref.
+    rewrite <- strategy_clight_ref. clear strategy_clight_ref.
+    (* fixme *)
+    unfold h, sig_assoc_left, sig_assoc_right, st_assoc_right.
+    (* unfold state_sig. *)
+
+    rewrite !slift_compose.
+    rewrite <- !compose_assoc. apply compose_proper_ref. 2: reflexivity.
+    rewrite !compose_assoc.
+    apply compose_proper_ref. reflexivity.
+    apply compose_proper_ref. reflexivity.
+    apply compose_proper_ref. reflexivity.
+    apply compose_proper_ref. reflexivity.
+    do 11 rewrite <- compose_assoc.
+    apply compose_proper_ref.
+    {
+      rewrite !compose_assoc.
+      unfold c_mem_state_rc.
+      rewrite <- !right_arrow_compose.
+      rewrite !compose_assoc.
+
+      rewrite <- (compose_assoc _ (right_arrow sig_assoc) (left_arrow sig_assoc)).
+      rewrite assoc_inverse. rewrite compose_unit_l.
+      setoid_rewrite <- (compose_assoc _ (left_arrow li_state_rc) (right_arrow li_state_rc)).
+      rewrite <- eta. rewrite compose_unit_l.
+      setoid_rewrite lift_rc_r.
+      setoid_rewrite <- (compose_assoc _ (slift (left_arrow c_rc)) (slift (right_arrow c_rc))).
+      rewrite <- (slift_compose (right_arrow c_rc)).
+      rewrite <- eta. rewrite slift_identity. rewrite compose_unit_l.
+      rewrite <- (compose_assoc _ (slift (left_arrow _)) (slift (right_arrow _))).
+      rewrite <- (slift_compose (right_arrow _) (left_arrow _)).
+      rewrite <- eta. rewrite slift_identity. rewrite compose_unit_l.
+      rewrite <- (compose_assoc _ _ (right_arrow sig_assoc)).
+      rewrite <- (compose_assoc _ (_ @ _)).
+      rewrite <- (compose_assoc _ (_ @ _)).
+      etransitivity.
+      instantiate (1 := slift (right_arrow r2) @
+                              right_arrow sig_assoc @ slift (slift (left_arrow r2))).
+      2: {
+        apply compose_proper_ref. reflexivity.
+        apply compose_proper_ref. 2: reflexivity.
+        apply assoc_property.
+      }
+      rewrite <- assoc_lift.
+      rewrite <- (compose_unit_l (right_arrow _)) at 1.
+      rewrite <- compose_assoc. apply compose_proper_ref. 2: reflexivity.
+      rewrite <- slift_compose. rewrite <- eta.
+      rewrite slift_identity. reflexivity.
+    }
+    rewrite <- (compose_unit_r (slift Sigma)) at 1.
+    apply compose_proper_ref. reflexivity.
+    unfold c_mem_state_rc. rewrite <- !left_arrow_compose.
+    rewrite !compose_assoc. cbn.
+    rewrite <- (compose_assoc _ ((left_arrow _)) ((right_arrow _))).
+    rewrite <- eta. rewrite compose_unit_l.
+    rewrite <- (compose_assoc _ ((right_arrow _)) ((left_arrow _))).
+    rewrite assoc_inverse. rewrite compose_unit_l.
+    setoid_rewrite lift_rc_l.
+    rewrite <- (compose_assoc _ (_ (left_arrow _)) (_ (right_arrow _))).
+    rewrite <- slift_compose. rewrite <- eta.
+    rewrite slift_identity. rewrite compose_unit_l.
+    rewrite <- slift_compose. rewrite <- eta.
+    rewrite slift_identity. reflexivity.
+  Qed.
+
+End COMPILE_LAYER.
+
+
+(** Obsolete stuff *)
+(*
+Local Opaque normalize_rc.
+Close Scope Z_scope.
+
+Lemma foo {E: esig} {S1 S2 S3 U: Type} (R: S1 -> S2 * S3 -> Prop):
+  right_arrow sig_comm @ slift (right_arrow (rc_id * rel_rc R)) [=
+    right_arrow (rc_id(E:=E#U) * rel_rc R) @ right_arrow sig_comm.
+Proof.
+  intros ? [ ? ? [ ? ? m [ u ] ] [ s1 ] ]. cbn.
+  unfold compose, rc_adj_right.
+  inf_intro ?. inf_intro m'. inf_intro [ Rx HRx ].
+  rc_destruct HRx. rc_destruct H. rc_destruct H0.
+  destruct m0 as [ ? ? e [ s ]].
+  eapply inf_at. inf_mor. eapply inf_at. inf_mor. eapply finf_at.
+  { rc_econstructor. }
+  intm.
+  inf_intro ?. inf_intro m'. inf_intro [ Ry HRy ].
+  rc_inversion HRy. depsubst. clear_hyp. clear Hrel.
+  eapply inf_at. inf_mor. eapply inf_at. inf_mor. eapply finf_at.
+  { rc_econstructor; rc_econstructor; eauto. }
+  intm. apply bind_proper_ref. 2: reflexivity.
+  intros [ ? ? ].
+  sup_intro [ n Hn ]. inv Hn. destruct n. destruct p.
+  cbn [fst snd] in *. subst. eapply fsup_at.
+  { apply Hsub2. constructor. }
+  fcd_simpl.
+  sup_intro [ n Hn ]. inv Hn.
+  eapply fsup_at.
+  { apply Hsub. instantiate (1 := (_, _)). split; eauto.
+    apply Hsub0. reflexivity. }
+  fcd_simpl. reflexivity.
+Qed.
+
+Lemma baz {E F: esig} {S1 S2} (f: E ~> F):
+  slift(S:=S1) (slift(S:=S2) f) [= right_arrow sig_comm @ slift(S:=S2) (slift(S:=S1) f) @ right_arrow sig_comm.
+Proof.
+Abort.
+
+Lemma xxx {E F: esig} {S1 S2} (f: E ~> F):
+  slift(S:=S1) (slift(S:=S2) f) [=
+    left_arrow sig_comm @ left_arrow sig_assoc @ (slift f) @ right_arrow sig_assoc @ right_arrow sig_comm.
+Proof.
+Abort.
+*)
